protocols/PORExtended.v
@@ -1,0 +1,786 @@
+(* DISTRIBUTION STATEMENT A. Approved for public release. Distribution is unlimited.
+ *
+ * This material is based upon work supported by the Department of the Air Force under Air Force
+ * Contract No. FA8702-15-D-0001. Any opinions, findings, conclusions or recommendations expressed
+ * in this material are those of the author(s) and do not necessarily reflect the views of the
+ * Department of the Air Force.
+ *
+ * © 2020 Massachusetts Institute of Technology.
+ *
+ * MIT Proprietary, Subject to FAR52.227-11 Patent Rights - Ownership by the contractor (May 2014)
+ *
+ * The software/firmware is provided to you on an As-Is basis
+ *
+ * Delivered to the U.S. Government with Unlimited Rights, as defined in DFARS Part 252.227-7013
+ * or 7014 (Feb 2014). Notwithstanding any copyright notice, U.S. Government rights in this work are
+ * defined by DFARS 252.227-7013 or DFARS 252.227-7014 as detailed above. Use of this work other than
+ * as specifically authorized by the U.S. Government may violate any copyrights that exist in this work. *)
+
+From Coq Require Import
+     Classical
+     Morphisms
+     JMeq
+     List.
+
+From KeyManagement Require Import
+     MyPrelude
+     Common
+     Automation
+     Maps
+     Keys
+     KeysTheory
+     Messages
+     MessageEq
+     MessageEqTheory
+     Tactics
+     Simulation
+     RealWorld
+     InvariantsTheory
+     AdversaryUniverse
+     AdversarySafety
+     UsersTheory.
+
+From protocols Require Import
+     RealWorldStepLemmas
+     ExampleProtocols
+     ModelCheck
+     ProtocolAutomation
+     SafeProtocol
+     SyntacticallySafe
+     LabelsAlign
+     PartialOrderReduction
+.
+
+Definition stuck_model_step_user_stuck_user {t__hon t__adv}
+           (st : universe t__hon t__adv * IdealWorld.universe t__hon) : Prop :=
+  forall uid u,
+    (fst st).(users) $? uid = Some u
+    -> (forall st', model_step_user uid st st' -> False)
+    -> (forall lbl bd, step_user lbl (Some uid) (build_data_step (fst st) u) bd -> False).
+
+
+Lemma user_step_label_deterministic :
+  forall A B C lbl1 lbl2 bd bd1' bd2' suid,
+    @step_user A B C lbl1 suid bd bd1'
+    -> step_user lbl2 suid bd bd2'
+    -> lbl1 = lbl2.
+Proof.
+  induction 1; invert 1;
+    subst;
+    eauto;
+    repeat
+      match goal with
+      | [ H : _ = _ |- _ ] => invert H; try contradiction
+      end;
+    eauto.
+
+  invert H.
+  invert H6.
+Qed.
+
+Lemma stuck_model_step_user_stuck_user_implies_labels_align :
+  forall t__hon t__adv st,
+    @stuck_model_step_user_stuck_user t__hon t__adv st
+    -> labels_align st.
+Proof.
+  unfold stuck_model_step_user_stuck_user, labels_align;
+    destruct st as [ru iu]; intros.
+
+  invert H0.
+  specialize (H _ _ H1).
+
+  destruct (classic (exists st, model_step_user u_id (ru,iu) st)).
+  - split_ex.
+    invert H0;
+      destruct ru, userData, userData0;
+      unfold build_data_step in *;
+      simpl in *;
+      clean_map_lookups.
+
+    + admit.  (* contradiction based on steps being deterministic *)
+    + 
+
+
+
+
+  - assert (forall st', ~ model_step_user u_id (ru,iu) st') by eauto using all_not_not_ex.
+    eapply H in H3; eauto.
+    contradiction.
+Qed.
+  
+
+
+Lemma stuck_other_step_not_unstuck :
+  forall t__hon t__adv uid st st',
+    @model_step_user t__hon t__adv uid st st'
+    -> forall uid' lbl u bd,
+      (fst st).(users) $? uid' = Some u
+      -> step_user lbl (Some uid') (build_data_step (fst st) u) bd
+      -> uid <> uid'
+      -> (forall st'', model_step_user uid' st st'' -> False)
+      -> (forall st'', model_step_user uid' st' st'' -> False).
+Proof.
+  intros.
+  invert H;
+    unfold build_data_step, buildUniverse in *; simpl in *.
+
+  - 
+  
+  invert H; invert H2;
+    unfold build_data_step, buildUniverse in *; simpl in *;
+      clean_map_lookups.
+  - destruct ru , userData, userData0; simpl in *.
+
+
+    assert (exists m, users $? uid' =
+                 Some
+                   {|
+                     key_heap := key_heap0;
+                     protocol := protocol0;
+                     msg_heap := msg_heap0 ++ m;
+                     c_heap := c_heap0;
+                     from_nons := from_nons0;
+                     sent_nons := sent_nons0;
+                     cur_nonce := cur_nonce0 |}).
+    eapply step_back_into_other_user with (u_id1 := uid) in H4; eauto.
+    split_ors; split_ex; eauto.
+
+    2: {
+      simpl.
+    
+
+
+
+Lemma stuck_other_step_not_unstuck :
+  forall t__hon t__adv t suid bd bd',
+
+    step_user Silent suid bd bd'
+    
+    -> forall (usrs usrs' : honest_users t__hon) (adv adv' : user_data t__adv) (cmd cmd' : user_cmd t)
+        cs cs' gks gks' ks ks' qmsgs qmsgs' mycs mycs' froms froms' sents sents' n n' uid ru iu,
+
+      bd = (usrs,adv,cs,gks,ks,qmsgs,mycs,froms,sents,n,cmd)
+      -> bd' = (usrs',adv',cs',gks',ks',qmsgs',mycs',froms',sents',n',cmd')
+      -> suid = Some uid
+      -> forall cmda1, usrs $? uid = Some (mkUserData ks cmda1 qmsgs mycs froms sents n)
+      -> ru = {| users := usrs; adversary := adv; all_ciphers := cs ; all_keys := gks |}
+      -> forall ru' uid' cmda,
+          uid <> uid'
+          -> (forall st, model_step_user uid' (ru,iu) st -> False)
+          -> ru' = buildUniverse_step (usrs',adv',cs',gks',ks',qmsgs',mycs',froms',sents',n',cmda) uid
+          -> (forall st, model_step_user uid' (ru',iu) st -> False).
+Proof.
+  induction 1; inversion 1; inversion 1; intros; subst;
+    eauto.
+
+  admit.
+  admit.
+
+  unfold buildUniverse_step in *; simpl in *.
+    
+
+
+Lemma stuck_step_implies_stuck_universe_step_labels_align :
+  forall t__hon t__adv st,
+    @stuck_step_implies_stuck_universe_step t__hon t__adv st
+    -> labels_align st.
+Proof.
+  destruct st as [ru iu].
+  unfold stuck_step_implies_stuck_universe_step, labels_align; intros.
+
+  destruct (classic (forall st', step (ru,iu) st' -> False)).
+  - exfalso; eauto.
+  - eapply not_all_not_ex in H1; split_ex.
+    
+
+Admitted.
+
+Lemma stuck_step_trsys_implies_labels_align :
+  forall t__hon t__adv st st',
+    (@step t__hon t__adv) ^* st st'
+    -> forall ru0 iu0,
+      st = (ru0,iu0)
+      -> invariantFor (@S t__hon t__adv ru0 iu0) stuck_step_implies_stuck_universe_step
+      -> labels_align st'.
+Proof.
+  induction 1; intros; subst; eauto.
+  - unfold invariantFor in *; simpl in *; intros.
+    assert (ARG : (ru0,iu0) = (ru0,iu0) \/ False) by eauto.
+    specialize (H0 _ ARG); clear ARG.
+    assert (STEP : (@step t__hon t__adv) ^* (ru0,iu0) (ru0,iu0)) by eauto.
+    apply H0 in STEP.
+    apply stuck_step_implies_stuck_universe_step_labels_align in STEP.
+    unfold labels_align in STEP; eauto.
+
+  - destruct y as [ru1 iu1].
+    assert (STEP : (@step t__hon t__adv) ^* (ru0,iu0) (ru1,iu1)) by (eapply TrcFront; eauto).
+    assert (INIT : (ru0,iu0) = (ru0,iu0) \/ False ) by eauto.
+
+    assert (INV : invariantFor (S ru1 iu1) stuck_step_implies_stuck_universe_step).
+    unfold invariantFor; simpl; intros.
+    destruct H1; try contradiction; subst.
+    eapply trc_trans in H3; eauto.
+    eapply H2; simpl; eauto.
+
+    eapply IHtrc in INV; eauto.
+Qed.
+
+Lemma stuck_step_violation_implies_alignment_violation :
+  forall t__hon t__adv st,
+    ~ @stuck_step_implies_stuck_universe_step t__hon t__adv st
+    -> ~ labels_align st.
+Proof.
+  unfold stuck_step_implies_stuck_universe_step, labels_align; intros.
+  destruct st as [ru iu]; simpl in *.
+  unfold not; intros.
+  eapply H; intros; clear H.
+  destruct lbl.
+  - eapply H1; econstructor; eauto.
+  - generalize H2; intros; eapply H0 in H2; split_ex.
+    eapply H1; econstructor 2; eauto.
+Qed.
+
+
+Module Type SyntacticallySafeProtocol.
+
+  Parameter t__hon : type.
+  Parameter t__adv : type.
+  Parameter b : << Base t__adv >>.
+  Parameter iu0 : IdealWorld.universe t__hon.
+  Parameter ru0 : RealWorld.universe t__hon t__adv.
+
+  Notation SYS := (S ru0 iu0).
+
+  Axiom U_good : universe_starts_sane b ru0.
+  Axiom universe_starts_safe : universe_ok ru0 /\ adv_universe_ok ru0 /\ syntactically_safe_U ru0.
+
+  Axiom safe_invariant : invariantFor
+                           SYS
+                           (fun st => no_resends_U (fst st)
+                                 /\ stuck_step_implies_stuck_universe_step st ).
+
+End SyntacticallySafeProtocol.
+
+Module ProtocolSimulates (Proto : SyntacticallySafeProtocol).
+  Import Proto.
+
+  Lemma no_resends_inv : invariantFor SYS (fun st => no_resends_U (fst st)).
+  Proof. eapply invariant_weaken; [ apply safe_invariant | firstorder idtac]. Qed.
+
+  Lemma stuck_not_misaligned_inv : invariantFor SYS stuck_step_implies_stuck_universe_step.
+  Proof. eapply invariant_weaken; [ apply safe_invariant | firstorder idtac]. Qed.
+
+  Hint Resolve no_resends_inv stuck_not_misaligned_inv.
+
+  Definition reachable_from := (fun ru iu ru' iu' => SYS.(Step)^* (ru, iu) (ru', iu')).
+  (* Definition reachable_froms := (fun st st' => reachable_from (fst st) (snd st) (fst st') (snd st')). *)
+  Definition reachable := (fun ru iu => reachable_from ru0 iu0 ru iu).
+  (* Definition reachables := (fun st => reachable (fst st) (snd st)). *)
+
+  Tactic Notation "invar" constr(invar_lem) :=
+    eapply use_invariant
+    ; [ eapply invar_lem
+      | eauto
+      |]
+    ; simpl
+    ; eauto.
+
+  Tactic Notation "invar" :=
+    eapply use_invariant
+    ; [ eauto .. |]
+    ; simpl
+    ; eauto.
+
+
+  Inductive R :
+    RealWorld.simpl_universe t__hon
+    -> IdealWorld.universe t__hon
+    -> Prop :=
+  | RStep : forall ru iu,
+      SYS.(Step) ^* (ru0,iu0) (ru,iu)
+      -> R (@RealWorld.peel_adv _ t__adv ru) iu.
+
+  Lemma single_step_stays_lame :
+    forall st st',
+      SYS.(Step) st st'
+      -> lameAdv b (adversary (fst st))
+      -> lameAdv b (adversary (fst st')).
+  Proof.
+    intros.
+    invert H;
+      simpl in *;
+      eauto using universe_step_preserves_lame_adv.
+  Qed.
+  
+  Lemma always_lame' :
+    forall st st',
+      SYS.(Step) ^* st st'
+      -> forall (ru ru' : RealWorld.universe t__hon t__adv) (iu iu' : IdealWorld.universe t__hon),
+          st = (ru,iu)
+        -> st' = (ru',iu')
+        -> lameAdv b (adversary ru)
+        -> lameAdv b (adversary ru').
+  Proof.
+    unfold SYS; simpl; intros *; intro H.
+    eapply trc_ind with (P:=fun st st' => lameAdv b (adversary (fst st)) -> lameAdv b (adversary (fst st'))) in H;
+      intros;
+      subst;
+      simpl in *;
+      eauto.
+  Qed.
+
+  Lemma always_lame :
+    forall (ru ru' : RealWorld.universe t__hon t__adv) (iu iu' : IdealWorld.universe t__hon),
+      lameAdv b (adversary ru)
+      -> SYS.(Step) ^* (ru,iu) (ru',iu')
+      -> lameAdv b (adversary ru').
+  Proof.
+    intros; eauto using always_lame'.
+  Qed.
+
+  Hint Resolve always_lame : safe.
+
+  Lemma lame_adv_no_impact_silent_step' :
+    forall A B C u_id bd bd',
+      step_user Silent (Some u_id) bd bd'
+      -> forall (usrs usrs' : honest_users A) (adv adv' advx : user_data B) (cmd cmd' : user_cmd C)
+          cs cs' gks gks' ks ks' qmsgs qmsgs' mycs mycs' froms froms' sents sents' n n',
+        bd = (usrs,adv,cs,gks,ks,qmsgs,mycs,froms,sents,n,cmd)
+        -> bd' = (usrs',adv',cs',gks',ks',qmsgs',mycs',froms',sents',n',cmd')
+        -> exists advx',
+            step_user Silent (Some u_id)
+                      (usrs,advx,cs,gks,ks,qmsgs,mycs,froms,sents,n,cmd)
+                      (usrs',advx',cs',gks',ks',qmsgs',mycs',froms',sents',n',cmd').
+  Proof.
+    induction 1; inversion 1; inversion 1;
+      intros;
+      repeat match goal with
+             | [ H : (_,_,_,_,_,_,_,_,_,_,_) = _ |- _ ] => invert H
+             end;
+      try solve [eexists; subst; econstructor; eauto].
+
+    specialize (IHstep_user _ _ _ _ advx _ _ _ _ _ _ _ _ _ _ _ _ _ _ _ _ _ _ eq_refl eq_refl); split_ex.
+    eexists; eapply StepBindRecur; eauto.
+  Qed.
+
+  Lemma lame_adv_no_impact_silent_step :
+    forall A B C u_id
+      (usrs usrs' : honest_users A) (adv adv' advx : user_data B) (cmd cmd' : user_cmd C)
+      cs cs' gks gks' ks ks' qmsgs qmsgs' mycs mycs' froms froms' sents sents' n n',
+      step_user Silent (Some u_id)
+                (usrs,adv,cs,gks,ks,qmsgs,mycs,froms,sents,n,cmd)
+                (usrs',adv',cs',gks',ks',qmsgs',mycs',froms',sents',n',cmd')
+      -> exists advx',
+        step_user Silent (Some u_id)
+                  (usrs,advx,cs,gks,ks,qmsgs,mycs,froms,sents,n,cmd)
+                  (usrs',advx',cs',gks',ks',qmsgs',mycs',froms',sents',n',cmd').
+  Proof.
+    intros; eauto using lame_adv_no_impact_silent_step'.
+  Qed.
+
+  Lemma lame_adv_no_impact_labeled_step' :
+    forall A B C u_id bd bd' a__r,
+      step_user (Action a__r) (Some u_id) bd bd'
+      -> forall (usrs usrs' : honest_users A) (adv adv' advx : user_data B) (cmd cmd' : user_cmd C)
+          cs cs' gks gks' ks ks' qmsgs qmsgs' mycs mycs' froms froms' sents sents' n n',
+        bd = (usrs,adv,cs,gks,ks,qmsgs,mycs,froms,sents,n,cmd)
+        -> bd' = (usrs',adv',cs',gks',ks',qmsgs',mycs',froms',sents',n',cmd')
+        -> exists advx',
+            step_user (Action a__r) (Some u_id)
+                      (usrs,advx,cs,gks,ks,qmsgs,mycs,froms,sents,n,cmd)
+                      (usrs',advx',cs',gks',ks',qmsgs',mycs',froms',sents',n',cmd').
+  Proof.
+    induction 1; inversion 1; inversion 1;
+      intros;
+      repeat match goal with
+             | [ H : (_,_,_,_,_,_,_,_,_,_,_) = _ |- _ ] => invert H
+             end;
+      try solve [eexists; subst; econstructor; eauto].
+
+    specialize (IHstep_user _ _ _ _ advx _ _ _ _ _ _ _ _ _ _ _ _ _ _ _ _ _ _ eq_refl eq_refl); split_ex.
+    eexists; eapply StepBindRecur; eauto.
+  Qed.
+
+  Lemma lame_adv_no_impact_labeled_step :
+    forall A B C u_id a__r
+      (usrs usrs' : honest_users A) (adv adv' advx : user_data B) (cmd cmd' : user_cmd C)
+      cs cs' gks gks' ks ks' qmsgs qmsgs' mycs mycs' froms froms' sents sents' n n',
+      step_user (Action a__r) (Some u_id)
+                (usrs,adv,cs,gks,ks,qmsgs,mycs,froms,sents,n,cmd)
+                (usrs',adv',cs',gks',ks',qmsgs',mycs',froms',sents',n',cmd')
+      -> exists advx',
+        step_user (Action a__r) (Some u_id)
+                  (usrs,advx,cs,gks,ks,qmsgs,mycs,froms,sents,n,cmd)
+                  (usrs',advx',cs',gks',ks',qmsgs',mycs',froms',sents',n',cmd').
+  Proof.
+    intros; eauto using lame_adv_no_impact_labeled_step'.
+  Qed.
+
+  Lemma reachable_from_silent_step :
+    forall iu (ru U U' : RealWorld.universe t__hon t__adv),
+      SYS.(Step) ^* (ru0,iu0) (ru,iu)
+      -> step_universe U Silent U'
+      -> lameAdv b U.(adversary)
+      -> ru.(users) = U.(users)
+      -> ru.(all_ciphers) = U.(all_ciphers)
+      -> ru.(all_keys) = U.(all_keys)
+      -> exists U'',
+          step_universe ru Silent U''
+          /\ peel_adv U' = peel_adv U''.
+  Proof.
+    intros.
+    assert (lameAdv b ru.(adversary))
+      by (pose proof U_good; unfold universe_starts_sane, adversary_is_lame in *; split_ands; eauto with safe).
+    
+    destruct ru; destruct U; simpl in *; subst.
+    invert H0.
+    - destruct userData; unfold build_data_step in *; simpl in *.
+
+      eapply lame_adv_no_impact_silent_step in H3; split_ex.
+      eexists; split.
+      eapply StepUser; unfold build_data_step; eauto; simpl in *.
+      unfold buildUniverse, peel_adv; simpl; trivial.
+      
+    - unfold lameAdv, build_data_step in *; simpl in *.
+      rewrite H1 in H2.
+      invert H2.
+  Qed.
+  
+  Lemma reachable_from_labeled_step :
+    forall iu (ru U U' : RealWorld.universe t__hon t__adv) a__r,
+      SYS.(Step) ^* (ru0,iu0) (ru,iu)
+      -> step_universe U (Action a__r) U'
+
+      -> lameAdv b U.(adversary)
+      -> ru.(users) = U.(users)
+      -> ru.(all_ciphers) = U.(all_ciphers)
+      -> ru.(all_keys) = U.(all_keys)
+      -> exists U'',
+          step_universe ru (Action a__r) U''
+          /\ peel_adv U' = peel_adv U''.
+  Proof.
+    intros.
+    assert (lameAdv b ru.(adversary))
+      by (pose proof U_good; unfold universe_starts_sane, adversary_is_lame in *; split_ands; eauto with safe).
+    
+    destruct ru; destruct U; simpl in *; subst.
+    invert H0.
+
+    destruct userData; unfold build_data_step in *; simpl in *.
+
+    eapply lame_adv_no_impact_labeled_step in H3; split_ex.
+    eexists; split.
+    eapply StepUser; unfold build_data_step; eauto; simpl in *.
+    unfold buildUniverse, peel_adv; simpl; trivial.
+  Qed.
+
+  Lemma simsilent : simulates_silent_step (lameAdv b) R.
+  Proof.
+    hnf
+    ; intros * REL UOK AUOK LAME * STEP
+    ; invert REL.
+
+    generalize (reachable_from_silent_step _ _ _ _ H3 STEP LAME H H1 H2);
+      intros; split_ex.
+
+    eexists; split; eauto.
+    rewrite H4.
+    econstructor.
+
+    eapply trcEnd_trc.
+    generalize (trc_trcEnd H3); intros.
+    econstructor; eauto.
+    unfold SYS; simpl.
+    econstructor; eauto.
+    
+  Qed.
+
+  Lemma message_eq_adv_change :
+    forall {t t1 t2} (m__rw : crypto t) (m__iw : IdealWorld.message.message t)
+      (U U' : RealWorld.universe t1 t2) (U__i : IdealWorld.universe t1) ch_id,
+      message_eq m__rw U m__iw U__i ch_id
+      -> users U = users U'
+      -> all_ciphers U = all_ciphers U'
+      -> all_keys U = all_keys U'
+      -> message_eq m__rw U' m__iw U__i ch_id.
+  Proof.
+    intros * MEQ RWU RWC RWK.
+    invert MEQ; [ econstructor 1 | econstructor 2 ]
+    ; rewrite <- ?RWU, <- ?RWC, <- ?RWK
+    ; eauto.
+  Qed.
+
+  Hint Resolve message_eq_adv_change : safe.
+  Hint Constructors action_matches : safe.
+  
+  Lemma action_matches_adv_change :
+    forall {t1 t2} (U U' : RealWorld.universe t1 t2) (U__i : IdealWorld.universe t1) a__r a__i,
+      action_matches a__r U a__i U__i
+      -> users U = users U'
+      -> all_ciphers U = all_ciphers U'
+      -> all_keys U = all_keys U'
+      -> action_matches a__r U' a__i U__i.
+  Proof.
+    intros * AM RWU RWC RWK.
+    invert AM; eauto with safe.
+  Qed.
+
+  Lemma simlabeled : simulates_labeled_step (lameAdv b) R.
+  Proof.
+    hnf
+    ; intros * REL UOK AUOK LAME * STEP
+    ; invert REL.
+
+    generalize (reachable_from_labeled_step _ _ _ _ _ H3 STEP LAME H H1 H2);
+      intros; split_ex.
+
+    admit.
+    (* pose proof labels_align_inv. *)
+    (* unfold invariantFor, SYS in H5; simpl in H5. *)
+    (* assert ( (ru0,iu0) = (ru0,iu0) \/ False ) as ARG by eauto. *)
+    (* specialize (H5 _ ARG _ H3 _ _ H0). *)
+
+    (* split_ex. *)
+    (* do 3 eexists; rewrite H4; repeat apply conj; eauto. *)
+    (* - invert H7; eauto with safe. *)
+      
+    (* - econstructor. *)
+
+    (*   eapply trcEnd_trc. *)
+    (*   generalize (trc_trcEnd H3); intros. *)
+    (*   econstructor; eauto. *)
+    (*   unfold SYS; simpl. *)
+    (*   econstructor; eauto. *)
+  Admitted.
+
+  (* Lemma honest_cmds_safe_adv_change : *)
+  (*   forall {t1 t2} (U U' : RealWorld.universe t1 t2), *)
+  (*     honest_cmds_safe U *)
+  (*     -> users U = users U' *)
+  (*     -> all_ciphers U = all_ciphers U' *)
+  (*     -> all_keys U = all_keys U' *)
+  (*     -> honest_cmds_safe U'. *)
+  (* Proof. *)
+  (*   intros * HCS RWU RWC RWK. *)
+  (*   unfold honest_cmds_safe in * *)
+  (*   ; intros *)
+  (*   ; rewrite <- ?RWU, <- ?RWC, <- ?RWK in * *)
+  (*   ; eauto. *)
+  (* Qed. *)
+
+  (* Hint Resolve honest_cmds_safe_adv_change : safe. *)
+
+  Require Import Coq.Program.Equality.
+
+  Lemma foo :
+    forall A B t (cmd : user_cmd t) (usrs : honest_users A) (adv : user_data B) cs gks
+      uid ks qmsgs mycs froms sents n,
+        (forall lbl bd, ~ step_user lbl (Some uid) (usrs,adv,cs,gks,ks,qmsgs,mycs,froms,sents,n,cmd) bd)
+        -> forall t__n cmd1 (cmd2 : <<t__n>> -> user_cmd t),
+        cmd = Bind cmd1 cmd2
+        -> forall lbl' bd',
+          ~ step_user lbl' (Some uid) (usrs,adv,cs,gks,ks,qmsgs,mycs,froms,sents,n,cmd1) bd'.
+  Admitted.
+
+  Hint Resolve foo : core.
+    
+
+  (* Lemma predicates_imply_next_cmd_safe_no_step' : *)
+  (*   forall A B t (cmd : user_cmd t) (usrs : honest_users A) (adv : user_data B) cs gks *)
+  (*     uid ks qmsgs mycs froms sents n ctx styp, *)
+  (*     syntactically_safe uid ctx cmd styp *)
+  (*     -> typingcontext_sound ctx (findUserKeys usrs) cs uid *)
+  (*     -> (forall usrs' adv' cs' gks' ks' qmsgs' mycs' froms' sents' n' cmd' lbl, *)
+  (*           ~ step_user lbl (Some uid) *)
+  (*             (usrs,adv,cs,gks,ks,qmsgs,mycs,froms,sents,n,cmd) *)
+  (*             (usrs',adv',cs',gks',ks',qmsgs',mycs',froms',sents',n',cmd')) *)
+  (*     -> next_cmd_safe (findUserKeys usrs) cs uid froms sents cmd. *)
+  (* Proof. *)
+  (*   dependent induction cmd; *)
+  (*     unfold next_cmd_safe; intros; *)
+  (*       match goal with *)
+  (*       | [ H : nextAction _ _ |- _ ] => invert H *)
+  (*       end; *)
+  (*       eauto. *)
+
+  (*   - invert H0. *)
+  (*     eapply IHcmd *)
+  (*         (* (bd := (usrs0, adv0, cs0, gks0, ks0, qmsgs0, mycs0, froms0, sents0, cur_n, cmd0)) *) *)
+  (*       in H10; eauto.  *)
+  (*     apply H10 in H7; eauto. *)
+  (*     intros; eauto. *)
+  (*     unfold not; intros. *)
+  (*     eapply H2. *)
+  (*     admit. *)
+    
+    (* forall A B C lbl suid bd bd', *)
+    (*   step_user lbl suid bd bd' *)
+    (*   -> forall (usrs usrs' : honest_users A) (adv adv' : user_data B) (cmd cmd' : user_cmd C) *)
+    (*       cs cs' gks gks' ks ks' qmsgs qmsgs' mycs mycs' froms froms' sents sents' n n' u_id, *)
+    (*     suid = Some u_id *)
+    (*     -> bd = (usrs,adv,cs,gks,ks,qmsgs,mycs,froms,sents,n,cmd) *)
+    (*     -> bd' = (usrs',adv',cs',gks',ks',qmsgs',mycs',froms',sents',n',cmd') *)
+    (*     -> no_resends sents' *)
+    (*     -> forall ctx styp, syntactically_safe u_id ctx cmd styp *)
+    (*     -> typingcontext_sound ctx (findUserKeys usrs) cs u_id *)
+    (*     -> forall cmdc, usrs $? u_id = Some {| key_heap := ks; *)
+    (*                                      protocol := cmdc; *)
+    (*                                      msg_heap := qmsgs; *)
+    (*                                      c_heap   := mycs; *)
+    (*                                      from_nons := froms; *)
+    (*                                      sent_nons := sents; *)
+    (*                                      cur_nonce := n |} *)
+    (*     -> next_cmd_safe (findUserKeys usrs) cs u_id froms sents cmd. *)
+
+
+  
+  (* Lemma predicates_imply_next_cmd_safe_step : *)
+  (*   forall A B C lbl suid bd bd', *)
+  (*     step_user lbl suid bd bd' *)
+  (*     -> forall (usrs usrs' : honest_users A) (adv adv' : user_data B) (cmd cmd' : user_cmd C) *)
+  (*         cs cs' gks gks' ks ks' qmsgs qmsgs' mycs mycs' froms froms' sents sents' n n' u_id, *)
+  (*       suid = Some u_id *)
+  (*       -> bd = (usrs,adv,cs,gks,ks,qmsgs,mycs,froms,sents,n,cmd) *)
+  (*       -> bd' = (usrs',adv',cs',gks',ks',qmsgs',mycs',froms',sents',n',cmd') *)
+  (*       -> no_resends sents' *)
+  (*       -> forall ctx styp, syntactically_safe u_id ctx cmd styp *)
+  (*       -> typingcontext_sound ctx (findUserKeys usrs) cs u_id *)
+  (*       -> forall cmdc, usrs $? u_id = Some {| key_heap := ks; *)
+  (*                                        protocol := cmdc; *)
+  (*                                        msg_heap := qmsgs; *)
+  (*                                        c_heap   := mycs; *)
+  (*                                        from_nons := froms; *)
+  (*                                        sent_nons := sents; *)
+  (*                                        cur_nonce := n |} *)
+  (*       -> next_cmd_safe (findUserKeys usrs) cs u_id froms sents cmd. *)
+  (* Proof. *)
+  (*   induction 1; inversion 2; inversion 1; *)
+  (*     unfold next_cmd_safe; intros; subst; *)
+  (*       match goal with *)
+  (*       | [ H : nextAction _ _ |- _ ] => invert H *)
+  (*       end; *)
+  (*       match goal with *)
+  (*       | [ H : syntactically_safe _ _ _ _  |- _ ] => *)
+  (*         invert H; unfold typingcontext_sound in *; split_ex *)
+  (*       end; *)
+  (*       eauto. *)
+
+  (*   - eapply IHstep_user in H6; eauto. *)
+  (*     invert H3; eauto. *)
+  (*   - invert H5; eauto. *)
+  (*   - eapply H4 in H12; split_ex; subst; clear H4. *)
+  (*     clean_context. *)
+  (*     invert H10. *)
+  (*     apply H in H14. *)
+  (*     unfold msg_honestly_signed, msg_signing_key, msg_to_this_user, msg_destination_user, honest_keyb; *)
+  (*       context_map_rewrites; *)
+  (*       destruct (cipher_to_user x0 ==n cipher_to_user x0); *)
+  (*       try contradiction. *)
+  (*     repeat simple apply conj; eauto. *)
+
+  (*     econstructor; eauto. *)
+
+  (*     unfold msg_honestly_signed, msg_signing_key, honest_keyb; *)
+  (*       context_map_rewrites; *)
+  (*       trivial. *)
+
+  (*     (do 2 eexists); repeat simple apply conj; eauto. *)
+      
+  (*     unfold no_resends in H22. *)
+  (*     invert H22; eauto. *)
+
+  (*   - intros. *)
+  (*     eapply H14 in H5; split_ex; subst; split; eauto. *)
+  (* Qed. *)
+  
+      
+  Lemma simsafe : honest_actions_safe t__adv R.
+  Proof.
+    hnf
+    ; intros * REL UOK AUOK
+    ; invert REL.
+
+    pose proof no_resends_inv.
+    unfold invariantFor, SYS in H0; simpl in H0.
+    assert ( (ru0,iu0) = (ru0,iu0) \/ False ) as ARG by auto.
+    specialize (H0 _ ARG); clear ARG.
+
+    assert (syntactically_safe_U ru) by admit.
+    unfold syntactically_safe_U in *; simpl in *.
+    unfold honest_cmds_safe; intros; subst.
+    destruct u; simpl.
+    generalize H6; intros USRS; rewrite <- H in USRS.
+    specialize (H4 _ _ USRS); split_ex; simpl in *.
+
+    rename U__i into iu.
+    destruct (classic (exists st', step (ru,iu) st')).
+    - split_ex.
+      rename x1 into st'.
+      assert (STEP : (@step t__hon t__adv) ^* (ru,iu) st') by (eauto using TrcFront).
+      pose proof (trc_trans H3 STEP) as STEPS.
+
+      specialize (H0 _ STEPS); unfold no_resends_U in H0.
+      
+      (* rewrite Forall_natmap_forall in H0; specialize (H0 _ _ USRS); simpl in H0. *)
+      (* eapply predicates_imply_next_cmd_safe; eauto. *)
+      admit.
+    - admit.
+
+
+    (* pose proof safety_inv. *)
+    (* unfold invariantFor, SYS in H0; simpl in H0. *)
+    (* assert ( (ru0,iu0) = (ru0,iu0) \/ False ) as ARG by eauto. *)
+    (* specialize (H0 _ ARG _ H3). *)
+    (* unfold safety in *; eauto with safe. *)
+
+  Admitted.
+
+  Hint Resolve simsilent simlabeled simsafe : safe.
+
+  Lemma proto_lamely_refines :
+    refines (lameAdv b) ru0 iu0.
+  Proof.
+    exists R; unfold simulates.
+
+    pose proof safe_invariant.
+    pose proof universe_starts_safe; split_ands.
+    
+    unfold invariantFor in H; simpl in H.
+    assert ( (ru0,iu0) = (ru0,iu0) \/ False ) as ARG by eauto.
+    specialize (H _ ARG); clear ARG.
+
+    Hint Constructors R : safe.
+
+    unfold simulates_silent_step, simulates_labeled_step;
+      intuition eauto with safe.
+
+  Qed.
+
+  Hint Resolve proto_lamely_refines : safe.
+
+  Lemma proto_starts_ok : universe_starts_ok ru0.
+  Proof.
+    pose proof universe_starts_safe.
+    pose proof U_good.
+    unfold universe_starts_ok; intros.
+    unfold universe_ok, adv_universe_ok, universe_starts_sane in *; split_ands.
+    intuition eauto.
+  Qed.
+
+  Hint Resolve proto_starts_ok : safe.
+
+  Theorem protocol_with_adversary_could_generate_spec :
+    forall U__ra advcode acts__r,
+      U__ra = add_adversary ru0 advcode
+      -> rCouldGenerate U__ra acts__r
+      -> exists acts__i,
+          iCouldGenerate iu0 acts__i
+          /\ traceMatches acts__r acts__i.
+  Proof.
+    intros.
+    pose proof U_good as L; unfold universe_starts_sane, adversary_is_lame in L; split_ands.
+    eapply refines_could_generate; eauto with safe.
+  Qed.
+
+End ProtocolSimulates.
+
